theories/Template/QuoteGround/Coq/Lists.v
@@ -1,0 +1,53 @@
+Require Import Coq.Lists.List.
+Require Import Coq.Lists.ListDec.
+From MetaCoq.Lob.Template Require Export QuoteGround.Coq.Init.
+Import ListNotations.
+Local Open Scope list_scope.
+
+(* not decidable *)
+(*
+#[export] Instance quote_Add {A a ls1 ls2} {qA : quotation_of A} {quoteA : ground_quotable A} : ground_quotable (@Add A a ls1 ls2) := ltac:(destruct 1; exact _). (a:A) : list A -> list A -> Prop :=
+#[export] Instance quote_NoDup {A} {qA : quotation_of A} {quoteA : ground_quotable A} {quote_neg_In : forall (a : A) ls, ground_quotable (~In a ls)} {ls} : ground_quotable (@NoDup A ls).
+Proof.
+  induction ls; adjust_ground_quotable_by_econstructor_inversion ().
+Defined.
+#[export] Instance quote_Exists : ground_quotable Exists := ltac:(destruct 1; exact _). : list A -> Prop :=
+ *)
+#[export] Instance quote_Forall {A R ls} {qA : quotation_of A} {qR : quotation_of R} {quoteA : ground_quotable A} {quoteR : forall x, ground_quotable (R x:Prop)} : ground_quotable (@Forall A R ls).
+Proof.
+  induction ls as [|a ls IH].
+  all: adjust_ground_quotable_by_econstructor_inversion ().
+Defined.
+#[export] Instance quote_Forall2 {A B R lsA lsB} {qA : quotation_of A} {qB : quotation_of B} {qR : quotation_of R} {quoteA : ground_quotable A} {quoteB : ground_quotable B} {quoteR : forall x y, ground_quotable (R x y:Prop)} : ground_quotable (@Forall2 A B R lsA lsB).
+Proof.
+  revert lsB; induction lsA as [|a lsA IH], lsB as [|b lsB].
+  all: try solve [ intro pf; exfalso; inversion pf ].
+  all: adjust_ground_quotable_by_econstructor_inversion ().
+Defined.
+#[export] Instance quote_ForallOrdPairs {A R ls} {qA : quotation_of A} {qR : quotation_of R} {quoteA : ground_quotable A} {quoteR : forall x y, ground_quotable (R x y:Prop)} : ground_quotable (@ForallOrdPairs A R ls).
+Proof.
+  induction ls as [|a ls IH].
+  all: adjust_ground_quotable_by_econstructor_inversion ().
+Defined.
+#[export] Instance quote_eqlistA {A R ls1 ls2} {qA : quotation_of A} {qR : quotation_of R} {quoteA : ground_quotable A} {quoteR : forall x y, ground_quotable (R x y:Prop)} : ground_quotable (@SetoidList.eqlistA A R ls1 ls2).
+Proof.
+  revert ls2; induction ls1 as [|a ls1 IH], ls2 as [|b ls2].
+  all: try solve [ intro pf; exfalso; inversion pf ].
+  all: adjust_ground_quotable_by_econstructor_inversion ().
+Defined.
+(*
+#[export] Instance quote_PermutationA : ground_quotable PermutationA := ltac:(destruct 1; exact _). : list A -> list A -> Prop :=
+ *)
+(*
+#[export] Instance quote_memo_val : ground_quotable memo_val := ltac:(destruct 1; exact _). {A : nat -> Type} : Type :=
+Co#[export] Instance quote_Stream : ground_quotable Stream := ltac:(destruct 1; exact _). (A : Type) :=
+Co#[export] Instance quote_EqSt : ground_quotable EqSt := ltac:(destruct 1; exact _). (s1 s2: Stream) : Prop :=
+#[export] Instance quote_Exists : ground_quotable Exists := ltac:(destruct 1; exact _). : Stream -> Prop :=
+#[export] Instance quote_Exists : ground_quotable Exists := ltac:(destruct 1; exact _). ( x: Stream ) : Prop :=
+Co#[export] Instance quote_ForAll : ground_quotable ForAll := ltac:(destruct 1; exact _). (x: Stream) : Prop :=
+*)
+
+Definition list_eq_nil_dec {A} {l : list A} : {l = []} + {l <> []}.
+Proof. destruct l; [ left | right ]; try reflexivity; congruence. Defined.
+#[export] Instance quote_list_neq_nil {A} {qA : quotation_of A} (l : list A) {ql : quotation_of l} : ground_quotable (l <> [])
+  := ground_quotable_neg_of_dec list_eq_nil_dec.
