theories/Template/QuoteGround/Coq/MSets.v
@@ -1,0 +1,192 @@
+From Coq Require Import MSetInterface MSetList MSetAVL MSetFacts MSetProperties MSetDecide.
+From MetaCoq.Lob.Util.Tactics Require Import
+     DestructHead.
+From MetaCoq.Lob.Template.QuoteGround Require Export Coq.Numbers Coq.Init.
+
+Module Type MSetAVL_MakeT (T : OrderedType). Include MSetAVL.Make T. End MSetAVL_MakeT.
+
+Module QuoteMSetAVL (T : OrderedType) (M : MSetAVL_MakeT T).
+  Module MFact := WFactsOn T M.
+  Module MProp := WPropertiesOn T M.
+  Module MDecide := WDecide (M).
+  Local Ltac msets := MDecide.fsetdec.
+
+  Scheme Induction for M.Raw.tree Sort Type.
+  Scheme Induction for M.Raw.tree Sort Set.
+  Scheme Induction for M.Raw.tree Sort Prop.
+  Scheme Case for M.Raw.tree Sort Type.
+  Scheme Case for M.Raw.tree Sort Prop.
+  Scheme Minimality for M.Raw.tree Sort Type.
+  Scheme Minimality for M.Raw.tree Sort Set.
+  Scheme Minimality for M.Raw.tree Sort Prop.
+
+  Fixpoint Raw_InT_dec x t : { M.Raw.InT x t } + {~ M.Raw.InT x t}.
+  Proof.
+    refine match t with
+           | M.Raw.Leaf => right _
+           | M.Raw.Node z l n r
+             => match T.compare x n as c, Raw_InT_dec x l, Raw_InT_dec x r return CompareSpec _ _ _ c -> _ with
+                | Eq, _, _ => fun pf => left (_ pf)
+                | _, left pf, _ => fun _ => left _
+                | _, _, left pf => fun _ => left _
+                | _, right p2, right p3 => fun p1 => right (_ p1)
+                end (T.compare_spec x n)
+           end;
+      try solve [ inversion 1
+                | inversion 1; first [ constructor; first [ assumption | subst; reflexivity ] | exfalso; discriminate ]
+                | constructor; assumption
+                | do 2 inversion 1; subst; exfalso;
+                  try congruence;
+                  match goal with
+                  | [ H : T.lt _ _, H' : T.eq _ _ |- False ]
+                    => rewrite H' in H; now eapply M.Raw.MX.lt_irrefl
+                  end ].
+  Defined.
+  Definition Raw_In_dec x y : {M.Raw.In x y} + {~M.Raw.In x y}.
+  Proof.
+    cbv [M.Raw.In]; apply Raw_InT_dec.
+  Defined.
+  Definition In_dec x y : {M.In x y} + {~M.In x y}.
+  Proof.
+    cbv [M.In]; apply Raw_In_dec.
+  Defined.
+  Definition Inb x y := b_of_dec (In_dec x y).
+  Definition Inb_bp x y : Inb x y = true -> M.In x y := bp_of_dec.
+  Definition Inb_pb x y : M.In x y -> Inb x y = true := pb_of_dec.
+
+  Section with_t.
+    Context {quote_T_t : ground_quotable T.t}.
+
+    #[export] Instance quote_M_Raw_t : ground_quotable M.Raw.t := (ltac:(induction 1; exact _)).
+    Fixpoint M_Raw_lt_tree_dec x t : { M.Raw.lt_tree x t } + {~ M.Raw.lt_tree x t}.
+    Proof.
+      refine match t with
+             | M.Raw.Leaf => left _
+             | M.Raw.Node z l n r
+               => match T.compare n x as c, M_Raw_lt_tree_dec x l, M_Raw_lt_tree_dec x r return CompareSpec _ _ _ c -> _ with
+                  | Lt, left p2, left p3 => fun pfc => left _
+                  | _, right pf, _ => fun pfc => right _
+                  | _, _, right pf => fun pfc => right _
+                  | _, _, _ => fun pfc => right _
+                  end (T.compare_spec _ _)
+             end;
+        try solve [ inversion 1; inversion pfc
+                  | inversion 1; inversion pfc; subst; auto;
+                    match goal with
+                    | [ H : T.lt _ _, H' : T.eq _ _ |- _ ]
+                      => now first [ rewrite -> H' in H | rewrite <- H' in H ]
+                    end
+                  | intro f; apply pf; hnf in *; intros; apply f; constructor; (assumption + reflexivity)
+                  | intro f; inversion pfc; eapply M.Raw.MX.lt_irrefl; (idtac + etransitivity); (eassumption + (eapply f; constructor; (idtac + symmetry); (eassumption + reflexivity))) ].
+    Defined.
+    Fixpoint M_Raw_gt_tree_dec x t : { M.Raw.gt_tree x t } + {~ M.Raw.gt_tree x t}.
+    Proof.
+      refine match t with
+             | M.Raw.Leaf => left _
+             | M.Raw.Node z l n r
+               => match T.compare n x as c, M_Raw_gt_tree_dec x l, M_Raw_gt_tree_dec x r return CompareSpec _ _ _ c -> _ with
+                  | Gt, left p2, left p3 => fun pfc => left _
+                  | _, right pf, _ => fun pfc => right _
+                  | _, _, right pf => fun pfc => right _
+                  | _, _, _ => fun pfc => right _
+                  end (T.compare_spec _ _)
+             end;
+        try solve [ inversion 1; inversion pfc
+                  | inversion 1; inversion pfc; subst; auto;
+                    match goal with
+                    | [ H : T.lt _ _, H' : T.eq _ _ |- _ ]
+                      => now first [ rewrite -> H' in H | rewrite <- H' in H ]
+                    end
+                  | intro f; apply pf; hnf in *; intros; apply f; constructor; (assumption + reflexivity)
+                  | intro f; inversion pfc; eapply M.Raw.MX.lt_irrefl; (idtac + etransitivity); (eassumption + (eapply f; constructor; (idtac + symmetry); (eassumption + reflexivity))) ].
+    Defined.
+    Fixpoint M_Raw_bst_dec t : { M.Raw.bst t } + {~ M.Raw.bst t}.
+    Proof.
+      refine match t with
+             | M.Raw.Leaf => left _
+             | M.Raw.Node z l n r
+               => match M_Raw_bst_dec l, M_Raw_bst_dec r, M_Raw_lt_tree_dec n l, M_Raw_gt_tree_dec n r with
+                  | right pf, _, _, _ => right _
+                  | _, right pf, _, _ => right _
+                  | _, _, right pf, _ => right _
+                  | _, _, _, right pf => right _
+                  | left p1, left p2, left p3, left p4 => left _
+                  end
+             end;
+        try solve [ constructor; assumption
+                  | inversion 1; subst; auto ].
+    Defined.
+    Definition M_Raw_bstb t := b_of_dec (M_Raw_bst_dec t).
+    Definition M_Raw_bstb_bst t : M_Raw_bstb t = true -> M.Raw.bst t := bp_of_dec.
+    Definition M_Raw_bstb_bst_alt t : M.Raw.bst t -> M_Raw_bstb t = true := pb_of_dec.
+    #[export] Instance quote_Raw_bst t : ground_quotable (M.Raw.bst t)
+      := ground_quotable_of_bp (@M_Raw_bstb_bst t) (@M_Raw_bstb_bst_alt t).
+    #[export] Instance quote_Raw_Ok s : ground_quotable (M.Raw.Ok s) := (ltac:(cbv [M.Raw.Ok]; exact _)).
+    #[export] Instance quote_t : ground_quotable M.t := (ltac:(induction 1; exact _)).
+
+    #[export] Instance quote_In x y : ground_quotable (M.In x y)
+      := ground_quotable_of_bp (@Inb_bp x y) (@Inb_pb x y).
+
+    Definition Raw_For_all_alt (P : M.elt -> Prop) : M.Raw.t -> Prop
+      := fix Raw_For_all_alt (s : M.Raw.t) : Prop
+        := match s with
+           | M.Raw.Leaf => True
+           | M.Raw.Node z l n r => Raw_For_all_alt l /\ P n /\ Raw_For_all_alt r
+           end.
+    Definition For_all_alt (P : M.elt -> Prop) (s : M.t) : Prop
+      := Raw_For_all_alt P (M.this s).
+    #[local] Hint Constructors M.Raw.InT : core typeclass_instances.
+    #[local] Hint Extern 1 (T.eq _ _) => reflexivity : core.
+    Lemma For_all_alt_iff P {P_Proper : Proper (T.eq ==> Basics.impl) P} s
+      : M.For_all P s <-> For_all_alt P s.
+    Proof using Type.
+      cbv [For_all_alt M.For_all M.In M.Raw.In M.this]; destruct s as [s _].
+      split; induction s; cbn; intro H'; auto; try inversion 1; subst; repeat apply conj; destruct_head'_and.
+      all: (idtac + (eapply P_Proper; (idtac + symmetry))); now eauto.
+    Defined.
+    Definition For_all_alt1 {P} {P_Proper : Proper (T.eq ==> Basics.impl) P} {s}
+      : M.For_all P s -> For_all_alt P s.
+    Proof. apply For_all_alt_iff; assumption. Defined.
+    Definition For_all_alt2 {P} {P_Proper : Proper (T.eq ==> Basics.impl) P} {s}
+      : For_all_alt P s -> M.For_all P s.
+    Proof. apply For_all_alt_iff; assumption. Defined.
+    #[export] Instance quote_For_all_alt {P s} {quote_P : forall x, M.In x s -> ground_quotable (P x:Prop)} {qP : quotation_of P} : ground_quotable (For_all_alt P s).
+    Proof.
+      cbv [For_all_alt M.For_all M.In M.Raw.In M.this] in *; destruct s as [s _].
+      induction s; cbn [Raw_For_all_alt]; try exact _.
+      apply @quote_and; try exact _.
+      2: apply @quote_and; try exact _.
+      all: eauto.
+    Defined.
+    #[export] Instance quote_For_all {P s} {quote_P : forall x, M.In x s -> ground_quotable (P x:Prop)} {qP : quotation_of P} {P_Proper : Proper (T.eq ==> Basics.impl) P} {qP_Proper : quotation_of P_Proper} : ground_quotable (M.For_all P s).
+    Proof.
+      intro pf.
+      let f := match goal with |- ?f _ => f end in
+      change (f (For_all_alt2 (For_all_alt1 pf))).
+      exact _.
+    Defined.
+  End with_t.
+End QuoteMSetAVL.
+
+(*
+Module Type MSetList_MakeWithLeibnizT (T : OrderedTypeWithLeibniz). Include MSetList.MakeWithLeibniz T. End MSetList_MakeWithLeibnizT.
+
+Module QuoteMSetListWithLeibniz (T : OrderedTypeWithLeibniz) (M : MSetList_MakeWithLeibnizT T).
+  Module MFact := WFactsOn T M.
+  Module MProp := WPropertiesOn T M.
+  Module MDecide := WDecide (M).
+  Local Ltac msets := MDecide.fsetdec.
+
+  Search M.In "dec".
+  Print MDecide.
+
+  Definition Raw_In_dec x y : {M.Raw.In x y} + {~M.Raw.In x y}.
+  Proof.
+    cbv [M.Raw.In]; apply InA_dec, T.eq_dec.
+  Defined.
+  Definition In_dec x y : {M.In x y} + {~M.In x y}.
+  Proof.
+    cbv [M.In]; apply Raw_In_dec.
+  Defined.
+End QuoteMSetListWithLeibniz.
+*)
