theories/Template/QuoteGround/Coq/Numbers.v
@@ -1,0 +1,6 @@
+Require Import Coq.Numbers.BinNums.
+From MetaCoq.Lob.Template Require Export QuoteGround.Coq.Init.
+
+#[export] Instance quote_positive : ground_quotable positive := ltac:(induction 1; exact _).
+#[export] Instance quote_N : ground_quotable N := ltac:(induction 1; exact _).
+#[export] Instance quote_Z : ground_quotable Z := ltac:(induction 1; exact _).
