theories/Template/QuoteGround/Init.v
@@ -1,0 +1,150 @@
+From MetaCoq.Template Require Import MonadBasicAst MonadAst All utils.
+Require Import Coq.Lists.List.
+Import ListNotations.
+
+Local Open Scope bs.
+Import MCMonadNotation.
+
+Class quotation_of {T} (t : T) := quoted_term_of : Ast.term.
+Class ground_quotable T := quote_ground : forall t : T, quotation_of t.
+Class debug_opt := debug : bool.
+
+Fixpoint replace_quotation_of {debug : debug_opt} (qt : term) : TemplateMonad term.
+Proof.
+  specialize (replace_quotation_of debug).
+  simple
+    refine
+    (let tmInferQuotation t
+       := (t <- tmUnquote t;;
+           let '(existT_typed_term _ t) := t in
+           v <- (tmInferInstance None (quotation_of t));;
+           match v with
+           | my_Some v => tmReturn v
+           | my_None => (if debug then tmPrint (quotation_of t) else tmReturn tt);; tmFail "No typeclass instance"
+           end) in
+     match qt return TemplateMonad Ast.term with
+     | tRel _
+     | tSort _
+     | tConstruct _ _ _
+     | tInt _
+     | tFloat _
+     | tConst _ _
+     | tInd _ _
+       => ret qt
+     | tVar id
+       => tmInferQuotation qt
+     | tEvar ev args => args <- monad_map replace_quotation_of args;; ret (tEvar ev args)
+     | tLambda na T M => T <- replace_quotation_of T;; M <- replace_quotation_of M;; ret (tLambda na T M)
+     | tApp u v => u <- replace_quotation_of u;; v <- monad_map replace_quotation_of v;; ret (mkApps u v)
+     | tProd na A B => A <- replace_quotation_of A;; B <- replace_quotation_of B;; ret (tProd na A B)
+     | tCast c kind ty => c <- replace_quotation_of c;; ty <- replace_quotation_of ty;; ret (tCast c kind ty)
+     | tLetIn na b ty b' => b <- replace_quotation_of b;; ty <- replace_quotation_of ty;; b' <- replace_quotation_of b';; ret (tLetIn na b ty b')
+     | tProj p c => replace_quotation_of c;; ret (tProj p c)
+     | tFix mfix idx =>
+         mfix' <- monad_map (monad_map_def (TM:=TypeInstance) replace_quotation_of replace_quotation_of) mfix;;
+         ret (tFix mfix' idx)
+     | tCoFix mfix idx =>
+         mfix' <- monad_map (monad_map_def (TM:=TypeInstance) replace_quotation_of replace_quotation_of) mfix;;
+         ret (tCoFix mfix' idx)
+     | tCase ind p c brs =>
+         p' <- monad_map_predicate (TM:=TypeInstance) ret replace_quotation_of replace_quotation_of p;;
+         brs' <- monad_map_branches (TM:=TypeInstance) replace_quotation_of brs;;
+         c <- replace_quotation_of c;;
+         ret (tCase ind p' c brs')
+     end); exact _.
+Defined.
+
+(** for fancier goals when we have [ground_quotable] for some subterms but not for subterms of those subterms *)
+Definition make_quotation_of {debug : debug_opt} {T} (t : T) : TemplateMonad (quotation_of t).
+Proof.
+  simple
+    refine
+    (qt <- tmQuote t;;
+     let tmInferQuotation t
+       := (t <- tmUnquote t;;
+           v <- (let '(existT_typed_term _ t) := t in tmInferInstance None (quotation_of t));;
+           match v with
+           | my_Some v => tmReturn v
+           | my_None => (if debug then tmPrint (quotation_of t) else tmReturn tt);; tmFail "No typeclass instance"
+           end) in
+     match qt return TemplateMonad Ast.term with
+     | tSort _
+     | tConst _ _
+     | tConstruct _ _ _
+     | tInt _
+     | tFloat _
+     | tInd _ _
+       => tmReturn qt
+     | tCast t kind v
+       => tmInferQuotation t
+     | tApp f args
+       => qf <- tmInferQuotation f;;
+          qargs <- list_rect
+                     (fun _ => _)
+                     (tmReturn [])
+                     (fun arg args qargs
+                      => qarg <- tmInferQuotation arg;;
+                         qargs <- qargs;;
+                         tmReturn (qarg :: qargs))
+                     args;;
+          tmReturn (tApp qf qargs)
+     | tProj proj t => tmFail "Proj is not reduced"
+     | tRel n => tmFail "Rel is not ground"
+     | tVar id => tmFail "Var is not ground"
+     | tEvar ev args => tmFail "Evar is not ground"
+     | tProd na ty body => tmFail "Prod not yet handled"
+     | tLambda na ty body => tmFail "Lambda not yet handled"
+     | tLetIn na def def_ty body => tmFail "LetIn not yet handled"
+     | tCase ci type_info discr branches => tmFail "Case not yet handled"
+     | tFix mfix idx => tmFail "Fix not yet handled"
+     | tCoFix mfix idx => tmFail "CoFix not yet handled"
+     end);
+    exact _.
+Defined.
+
+Ltac replace_quotation_of_goal _ :=
+  let G := match goal with |- quotation_of ?G => G end in
+  tryif is_var G
+  then fail "Avoiding loops"
+  else run_template_program (replace_quotation_of <% G %>) (fun v => exact v).
+
+Ltac make_quotation_of_goal _ :=
+  let t := match goal with |- quotation_of ?t => t end in
+  run_template_program (make_quotation_of t) (fun v => exact v).
+
+Ltac adjust_quotation_of_by_econstructor_then tac1 tac2 :=
+  let f := match goal with |- ?f _ => f end in
+  unshelve (let g := open_constr:(f _) in
+            change g);
+  [ unshelve econstructor
+  | ];
+  [ ..
+  | repeat match goal with |- context[?ev] => is_evar ev; generalize ev; intro end ];
+  [ tac1 () ..
+  | tac2 () ].
+
+Ltac adjust_ground_quotable_by_econstructor_inversion _ :=
+  let pf := fresh "pf" in
+  intro pf;
+  adjust_quotation_of_by_econstructor_then ltac:(fun _ => inversion pf; try assumption) ltac:(fun _ => try exact _).
+
+Module Export Instances.
+  #[export] Instance default_debug : debug_opt | 1000 := false.
+  #[export] Existing Instance quote_ground.
+  #[export] Typeclasses Opaque quotation_of.
+  #[export]
+   Hint Extern 1 (quotation_of match ?t with _ => _ end) => is_var t; destruct t : typeclass_instances.
+  #[export]
+   Hint Extern 1 (ground_quotable match ?t with _ => _ end) => is_var t; destruct t : typeclass_instances.
+  #[export]
+   Hint Extern 1 (quotation_of _) => replace_quotation_of_goal () : typeclass_instances.
+  #[export]
+   Hint Extern 2 (quotation_of ?t) => make_quotation_of_goal () : typeclass_instances.
+End Instances.
+
+Module StrongerInstances.
+  #[export]
+   Hint Extern 1 (quotation_of match ?t with _ => _ end) => destruct t : typeclass_instances.
+  #[export]
+   Hint Extern 1 (ground_quotable match ?t with _ => _ end) => destruct t : typeclass_instances.
+End StrongerInstances.
